theories/funext.v
@@ -1,0 +1,509 @@
+From Theories Require Import category.
+From Theories Require Import translation_fib.
+
+Set Primitive Projections.
+Set Universe Polymorphism.
+Set Polymorphic Inductive Cumulativity.
+
+
+(* translation of equality, CubicalTT-style *)
+
+Definition path0 {p}
+  (A0 : @El0 p Type0)
+  (A1 : @El1 p Type0 Type1 A0)
+  (x0 : El0 A0)
+  (x1 : El1 A0 A1 x0)
+  (y0 : El0 A0)
+  (y1 : El1 A0 A1 y0)
+: @El0 p Type0.
+Proof.
+refine (fun q α => _).
+unshelve econstructor.
+- refine (fun r β => _).
+  exact (itype r ((A0 r (α ∘ β)).(yft0) r !)
+    (x0 r (α ∘ β)) (y0 r (α ∘ β))).
+- refine (fun r β s => _). simpl in s.
+  refine
+  (forall (αi : r ≤ 1),
+  (A0 r (α ∘ β)).(yft1) r !
+  (fun r0 β0 => cast0 A0 A1 (α ∘ β) β0
+    _
+  )).
+  refine (itype_out (s r0 β0) (αi ∘ β0)).
+- refine (fun r β => _).
+  apply falso.
+Defined.
+
+Definition path1 {p}
+  (A0 : @El0 p Type0)
+  (A1 : @El1 p Type0 Type1 A0)
+  (x0 : El0 A0)
+  (x1 : El1 A0 A1 x0)
+  (y0 : El0 A0)
+  (y1 : El1 A0 A1 y0)
+: @El1 p Type0 Type1 (path0 A0 A1 x0 x1 y0 y1).
+Proof.
+refine (fun q α => _).
+reflexivity.
+Defined.
+
+Definition path_refl0 {p}
+  (A0 : @El0 p Type0)
+  (A1 : @El1 p Type0 Type1 A0)
+  (x0 : El0 A0)
+  (x1 : El1 A0 A1 x0)
+: El0 (path0 A0 A1 x0 x1 x0 x1).
+Proof.
+refine (fun q α => _). simpl.
+exact (itype_in (fun _ => x0 q α)).
+Defined.
+
+Definition path_refl1 {p}
+  (A0 : @El0 p Type0)
+  (A1 : @El1 p Type0 Type1 A0)
+  (x0 : El0 A0)
+  (x1 : El1 A0 A1 x0)
+: El1 _ (path1 A0 A1 x0 x1 x0 x1) (path_refl0 A0 A1 x0 x1).
+Proof.
+refine (fun q α αi => _).
+unfold path_refl0 ; simpl. unfold cast0 ; simpl.
+refine (J_seqs _ (fun p A x y => x y)
+  (fun X _ => yft1 (A0 q α) q !
+    (fun r β => J_seq _ (α ⋅ A0)
+      (fun a _ => yft0 (a r β) r !)
+      (X r (yft0 (A0 r (α ∘ β)) r !) (fun _ => x0 r (α ∘ β)) (αi ∘ β))
+      (fun r (β : r ≤ q) => yft_funct β (A0 q α)) (A1 q α)
+    )
+  )
+  _ (fun p A (x : p ≤ 1 -> A) y => itype_out (itype_in x) y)
+  (ssym itype_inout)).
+refine (x1 q α).
+Defined.
+
+Definition itype_out0_aux {p} {A : Type} {B : A -> SProp}
+  {X : forall (a : A) (b : B a), Type} {y z : forall (a : A) (b : B a), X a b}
+  {x : forall (a : A) (b : B a), itype p (X a b) (y a b) (z a b)} :
+  (fun a b => itype_out (x a b) i0) ≡ y.
+Proof.
+refine (J_seqs _ _ (fun T _ => (fun a b => T p (X a b) (y a b) (z a b) (x a b)) ≡ y) (srefl _) _ (ssym itype_out0)).
+Defined.
+
+Definition itype_out1_aux {p} {A : Type} {B : A -> SProp}
+  {X : forall (a : A) (b : B a), Type} {y z : forall (a : A) (b : B a), X a b}
+  {x : forall (a : A) (b : B a), itype p (X a b) (y a b) (z a b)} :
+  (fun a b => itype_out (x a b) i1) ≡ z.
+Proof.
+refine (J_seqs _ _ (fun T _ => (fun a b => T p (X a b) (y a b) (z a b) (x a b)) ≡ z) (srefl _) _ (ssym itype_out1)).
+Defined.
+
+Definition path_funext0 {p}
+  (A0 : @El0 p Type0)
+  (A1 : @El1 p Type0 Type1 A0)
+  (B0 : @El0 p Type0)
+  (B1 : @El1 p Type0 Type1 B0)
+  (f0 : El0 (Arr0 A0 A1 B0 B1))
+  (f1 : El1 _ (Arr1 A0 A1 B0 B1) f0)
+  (g0 : El0 (Arr0 A0 A1 B0 B1))
+  (g1 : El1 _ (Arr1 A0 A1 B0 B1) g0)
+  (h0 : El0 (Prod0 A0 A1
+    (fun q α x0 x1 => path0 (α ⋅ B0) (α ⋅ B1)
+      (app0 (α ⋅ f0) x0 x1) (app1 (α ⋅ f1) x0 x1)
+      (app0 (α ⋅ g0) x0 x1) (app1 (α ⋅ g1) x0 x1) q !)
+    (fun q α x0 x1 => path1 (α ⋅ B0) (α ⋅ B1)
+      (app0 (α ⋅ f0) x0 x1) (app1 (α ⋅ f1) x0 x1)
+      (app0 (α ⋅ g0) x0 x1) (app1 (α ⋅ g1) x0 x1) q !)
+    ))
+  (h1 : El1 _ (Prod1 A0 A1
+    (fun q α x0 x1 => path0 (α ⋅ B0) (α ⋅ B1)
+      (app0 (α ⋅ f0) x0 x1) (app1 (α ⋅ f1) x0 x1)
+      (app0 (α ⋅ g0) x0 x1) (app1 (α ⋅ g1) x0 x1) q !)
+    (fun q α x0 x1 => path1 (α ⋅ B0) (α ⋅ B1)
+      (app0 (α ⋅ f0) x0 x1) (app1 (α ⋅ f1) x0 x1)
+      (app0 (α ⋅ g0) x0 x1) (app1 (α ⋅ g1) x0 x1) q !)
+    ) h0)
+: El0 (path0 (Arr0 A0 A1 B0 B1) (Arr1 A0 A1 B0 B1) f0 f1 g0 g1).
+Proof.
+refine (fun q α => _).
+change (itype q (forall x0 : El0 (α ⋅ A0), El1 (α ⋅ A0) (α ⋅ A1) x0 -> yft0 (B0 q α) q !) (f0 q α) (g0 q α)).
+assert ((fun x0 x1 => itype_out (h0 q α x0 x1) i0) ≡ f0 q α) as H0.
+{ apply itype_out0_aux. }
+assert ((fun x0 x1 => itype_out (h0 q α x0 x1) i1) ≡ g0 q α) as H1.
+{ apply itype_out1_aux. }
+refine (J_seq _ _ (fun x _ => itype q _ x _) _ _ H0).
+refine (J_seq _ _ (fun x _ => itype q _ _ x) _ _ H1).
+refine (itype_in (fun αi x0 x1 => itype_out (h0 q α x0 x1) αi)).
+Defined.
+
+Lemma app2_seq {A : Type} {B : A -> Type} {C : forall (x : A) (y : B x), Type} {f g : forall (x : A) (y : B x), C x y} (e : f ≡ g) (x : A) (y : B x) : f x y ≡ g x y.
+Proof.
+refine (J_seqs _ _ (fun X _ => f x y ≡ X x y) (srefl _) _ e).
+Defined.
+
+Definition path_funext1 {p}
+  (A0 : @El0 p Type0)
+  (A1 : @El1 p Type0 Type1 A0)
+  (B0 : @El0 p Type0)
+  (B1 : @El1 p Type0 Type1 B0)
+  (f0 : El0 (Arr0 A0 A1 B0 B1))
+  (f1 : El1 _ (Arr1 A0 A1 B0 B1) f0)
+  (g0 : El0 (Arr0 A0 A1 B0 B1))
+  (g1 : El1 _ (Arr1 A0 A1 B0 B1) g0)
+  (h0 : El0 (Prod0 A0 A1
+    (fun q α x0 x1 => path0 (α ⋅ B0) (α ⋅ B1)
+      (app0 (α ⋅ f0) x0 x1) (app1 (α ⋅ f1) x0 x1)
+      (app0 (α ⋅ g0) x0 x1) (app1 (α ⋅ g1) x0 x1) q !)
+    (fun q α x0 x1 => path1 (α ⋅ B0) (α ⋅ B1)
+      (app0 (α ⋅ f0) x0 x1) (app1 (α ⋅ f1) x0 x1)
+      (app0 (α ⋅ g0) x0 x1) (app1 (α ⋅ g1) x0 x1) q !)
+    ))
+  (h1 : El1 _ (Prod1 A0 A1
+    (fun q α x0 x1 => path0 (α ⋅ B0) (α ⋅ B1)
+      (app0 (α ⋅ f0) x0 x1) (app1 (α ⋅ f1) x0 x1)
+      (app0 (α ⋅ g0) x0 x1) (app1 (α ⋅ g1) x0 x1) q !)
+    (fun q α x0 x1 => path1 (α ⋅ B0) (α ⋅ B1)
+      (app0 (α ⋅ f0) x0 x1) (app1 (α ⋅ f1) x0 x1)
+      (app0 (α ⋅ g0) x0 x1) (app1 (α ⋅ g1) x0 x1) q !)
+    ) h0)
+: El1 _ (path1 (Arr0 A0 A1 B0 B1) (Arr1 A0 A1 B0 B1) f0 f1 g0 g1)
+  (path_funext0 A0 A1 B0 B1 f0 f1 g0 g1 h0 h1).
+Proof.
+refine (fun q α αi x0 x1 => _).
+change (yft1 (B0 q α) q ! (fun r β => cast0 B0 B1 α β (itype_out (path_funext0 A0 A1 B0 B1 f0 f1 g0 g1 h0 h1 r (α ∘ β)) (αi ∘ β) (β ⋅ x0) (β ⋅ x1)))).
+unfold path_funext0 ; simpl.
+assert ((fun r β y0 y1 => itype_out (h0 r (α ∘ β) y0 y1) i0) ≡ (fun r β => f0 r (α ∘ β))) as H0.
+{ refine (J_seqs _ _ (fun T _ => (fun r β y0 y1 => T r (yft0 (B0 r (α ∘ β)) r !) (f0 r (α ∘ β) y0 y1) (g0 r (α ∘ β) y0 y1) (h0 r (α ∘ β) y0 y1)) ≡ α ⋅ f0) (srefl _) _ (ssym itype_out0)). }
+assert ((fun r β y0 y1 => itype_out (h0 r (α ∘ β) y0 y1) i1) ≡ (fun r β => g0 r (α ∘ β))) as H1.
+{ refine (J_seqs _ _ (fun T _ => (fun r β y0 y1 => T r (yft0 (B0 r (α ∘ β)) r !) (f0 r (α ∘ β) y0 y1) (g0 r (α ∘ β) y0 y1) (h0 r (α ∘ β) y0 y1)) ≡ α ⋅ g0) (srefl _) _ (ssym itype_out1)). }
+
+match goal with
+|- yft1 (B0 q α) q ! (fun r β => cast0 B0 B1 α β (itype_out (J_seq ?TT ?XX ?PP ?AA ?YY ?EE) (αi ∘ β) (β ⋅ x0) (β ⋅ x1))) =>
+refine (J_seqs _ (fun r β y0 y1 => itype_out (h0 r (α ∘ β) y0 y1) i0) (fun X E =>
+  yft1 (B0 q α) q ! (fun r β => cast0 B0 B1 α β (@itype_out r
+    (forall y0 y1, yft0 (B0 r (α ∘ β)) r !) (X r β) (g0 r (α ∘ β))
+    (J_seq TT (fun y0 y1 => itype_out (h0 r (α ∘ β) y0 y1) i0) PP AA (X r β) (app2_seq E r β))
+    (αi ∘ β) (β ⋅ x0) (β ⋅ x1))))
+  _ (fun r β => f0 r (α ∘ β)) H0)
+end.
+simpl.
+
+match goal with
+|- yft1 (B0 q α) q ! (fun r β => cast0 B0 B1 α β (itype_out (J_seq ?TT ?XX ?PP ?AA ?YY ?EE) (αi ∘ β) (β ⋅ x0) (β ⋅ x1))) =>
+refine (J_seqs _ (fun r β y0 y1 => itype_out (h0 r (α ∘ β) y0 y1) i1) (fun X E =>
+  yft1 (B0 q α) q ! (fun r β => cast0 B0 B1 α β (@itype_out r
+    (forall y0 y1, yft0 (B0 r (α ∘ β)) r !) (fun y0 y1 => itype_out (h0 r (α ∘ β) y0 y1) i0) (X r β)
+    (J_seq TT (fun y0 y1 => itype_out (h0 r (α ∘ β) y0 y1) i1) PP AA (X r β) (app2_seq E r β))
+    (αi ∘ β) (β ⋅ x0) (β ⋅ x1))))
+  _ (fun r β => g0 r (α ∘ β)) H1)
+end.
+simpl.
+
+refine (J_seqs _ (fun (p : ℙ) (A : Type) (x : (p ≤ 1) -> A) (y : p ≤ 1) => x y)
+               (fun X _ => yft1 (B0 q α) q ! (fun r β => cast0 B0 B1 α β (X r (forall y0 y1, yft0 (B0 r (α ∘ β)) r !) (fun αi0 x2 x3 => itype_out (h0 r (α ∘ β) x2 x3) αi0) (αi ∘ β) (β ⋅ x0) (β ⋅ x1))))
+               _ (fun p A (x : p ≤ 1 -> A) y => itype_out (itype_in x) y) (ssym itype_inout)).
+refine (h1 q α x0 x1 αi).
+Defined.
+
+(* comparing eq and path *)
+(* we get functions both ways, but they do not form an equivalence without funext/η, since
+   α ≠ merge (squish ∘ α) (antisquish ∘ α) *)
+
+Lemma itype_out0_aux2 {A : Type} {B : A -> Type}
+  {p : forall (a : A) (b : B a), nat}
+  {X : forall (a : A) (b : B a), Type} {y z : forall (a : A) (b : B a), X a b}
+  {x : forall (a : A) (b : B a), itype (p a b) (X a b) (y a b) (z a b)} :
+  (fun a b => itype_out (x a b) i0) ≡ y.
+Proof.
+refine (J_seqs _ _ (fun T _ => (fun a b => T (p a b) (X a b) (y a b) (z a b) (x a b)) ≡ y) (srefl _) _ (ssym itype_out0)).
+Defined.
+
+Lemma itype_out1_aux2 {A : Type} {B : A -> Type}
+  {p : forall (a : A) (b : B a), nat}
+  {X : forall (a : A) (b : B a), Type} {y z : forall (a : A) (b : B a), X a b}
+  {x : forall (a : A) (b : B a), itype (p a b) (X a b) (y a b) (z a b)} :
+  (fun a b => itype_out (x a b) i1) ≡ z.
+Proof.
+refine (J_seqs _ _ (fun T _ => (fun a b => T (p a b) (X a b) (y a b) (z a b) (x a b)) ≡ z) (srefl _) _ (ssym itype_out1)).
+Defined.
+
+Definition compare0 {p}
+  (A0 : @El0 p Type0)
+  (A1 : @El1 p Type0 Type1 A0)
+  (x0 : El0 A0)
+  (x1 : El1 A0 A1 x0)
+  (y0 : El0 A0)
+  (y1 : El1 A0 A1 y0)
+  (e0 : El0 (path0 A0 A1 x0 x1 y0 y1))
+  (e1 : El1 _ (path1 A0 A1 x0 x1 y0 y1) e0)
+  : El0 (eq0 A0 A1 x0 x1 y0 y1).
+Proof.
+refine (fun q α => _).
+unshelve econstructor.
+- refine (fun r β => _).
+  refine (itype_out (e0 r (α ∘ squish ∘ β)) (antisquish ∘ β)).
+- refine (fun r β => _).
+  refine (e1 r (α ∘ squish ∘ β) (antisquish ∘ β)).
+- change ((fun r β => itype_out (e0 r (α ∘ β)) i0) ≡ α ⋅ x0).
+  eapply itype_out0_aux2.
+- change ((fun r β => itype_out (e0 r (α ∘ β)) i1) ≡ α ⋅ y0).
+  eapply itype_out1_aux2.
+Defined.
+
+Definition compare1 {p}
+  (A0 : @El0 p Type0)
+  (A1 : @El1 p Type0 Type1 A0)
+  (x0 : El0 A0)
+  (x1 : El1 A0 A1 x0)
+  (y0 : El0 A0)
+  (y1 : El1 A0 A1 y0)
+  (e0 : El0 (path0 A0 A1 x0 x1 y0 y1))
+  (e1 : El1 _ (path1 A0 A1 x0 x1 y0 y1) e0)
+  : El1 _ (eq1 A0 A1 x0 x1 y0 y1) (compare0 A0 A1 x0 x1 y0 y1 e0 e1).
+Proof.
+refine (fun q α => _). simpl. unfold cube_eqR.
+reflexivity.
+Defined.
+
+Definition anticompare0 {p}
+  (A0 : @El0 p Type0)
+  (A1 : @El1 p Type0 Type1 A0)
+  (x0 : El0 A0)
+  (x1 : El1 A0 A1 x0)
+  (y0 : El0 A0)
+  (y1 : El1 A0 A1 y0)
+  (e0 : El0 (eq0 A0 A1 x0 x1 y0 y1))
+  (e1 : El1 _ (eq1 A0 A1 x0 x1 y0 y1) e0)
+  : El0 (path0 A0 A1 x0 x1 y0 y1).
+Proof.
+refine (fun q α => _). simpl.
+refine (J_seq _ _ (fun x _ => itype q _ (x q !) _) _ _ ((e0 q α).(ce_s))).
+refine (J_seq _ _ (fun x _ => itype q _ _ (x q !)) _ _ ((e0 q α).(ce_t))).
+refine (@itype_in q (yft0 (A0 q α) q !) (fun αi => (e0 q α).(ce_f0) q (merge ! αi))).
+Defined.
+
+Definition anticompare1 {p}
+  (A0 : @El0 p Type0)
+  (A1 : @El1 p Type0 Type1 A0)
+  (x0 : El0 A0)
+  (x1 : El1 A0 A1 x0)
+  (y0 : El0 A0)
+  (y1 : El1 A0 A1 y0)
+  (e0 : El0 (eq0 A0 A1 x0 x1 y0 y1))
+  (e1 : El1 _ (eq1 A0 A1 x0 x1 y0 y1) e0)
+  : El1 _ (path1 A0 A1 x0 x1 y0 y1) (anticompare0 A0 A1 x0 x1 y0 y1 e0 e1).
+Proof.
+refine (fun q α αi => _).
+change (yft1 (A0 q α) q ! (fun r β => cast0 A0 A1 α β (itype_out (anticompare0 A0 A1 x0 x1 y0 y1 e0 e1 r (α ∘ β)) (αi ∘ β)))).
+unfold anticompare0.
+pose proof (e1 q α). simpl in H. unfold cube_eqR in H. unfold cast0 in H. simpl in H.
+refine (J_seqs _ _ (fun X _ =>
+  yft1 (A0 q α) q ! (fun r β => cast0 A0 A1 α β (itype_out
+    (J_seq _ _
+      (fun x (_ : side_0 ⋅ ce_f0 (X r β) ≡ x) =>
+        itype r (yft0 (A0 r (α ∘ β)) r !)
+          (x r !) (y0 r ((α ∘ β) ∘ !)))
+      (J_seq _ _
+        (fun x (_ : side_1 ⋅ ce_f0 (X r β) ≡ x) =>
+          itype r (yft0 (A0 r (α ∘ β)) r !)
+            (ce_f0 (X r β) r side_0) (x r !))
+        (@itype_in r (yft0 (A0 r (α ∘ β)) r !) (fun αi0 : r ≤ 1 => ce_f0 (X r β) r (merge ! αi0)))
+        (α ∘ β ⋅ y0) (ce_t (X r β)))
+      (α ∘ β ⋅ x0) (ce_s (X r β)))
+    (αi ∘ β)))) _ _ (ssym H)). simpl.
+pose proof (ce_t (e0 q α)).
+refine (J_seqs _ _ (fun X E =>
+  yft1 (A0 q α) q !
+    (fun (r : nat) (β : r ≤ q) =>
+     cast0 A0 A1 α β
+       (itype_out
+          (J_seq _ _
+             (fun (x : forall (x2 : nat) (x3 : x2 ≤ r), yft0 (A0 x2 ((α ∘ β) ∘ (squish ∘ (side_0 ∘ x3)))) x2 !)
+                (_ : (fun (r0 : nat) (β0 : r0 ≤ r) => ce_f0 (e0 q (α ∘ !)) r0 (promote β ∘ (side_0 ∘ β0))) ≡ x)
+              => itype r (yft0 (A0 r (α ∘ β)) r !) (x r !) (X r β))
+             (J_seq _ _
+                (fun
+                   (x : forall (x2 : nat) (x3 : x2 ≤ r), yft0 (A0 x2 ((α ∘ β) ∘ (squish ∘ (side_1 ∘ x3)))) x2 !)
+                   (_ : (fun (r0 : nat) (β0 : r0 ≤ r) => ce_f0 (e0 q (α ∘ !)) r0 (promote β ∘ (side_1 ∘ β0))) ≡ x)
+                 => itype r (yft0 (A0 r (α ∘ β)) r !) (ce_f0 (e0 q (α ∘ !)) r (promote β ∘ side_0)) (x r !))
+                (@itype_in r (yft0 (A0 r (α ∘ β)) r !)
+                   (fun αi0 : r ≤ 1 => ce_f0 (e0 q (α ∘ !)) r (promote β ∘ merge ! αi0)))
+                (β ⋅ X)
+                (J_seqs _ _
+                   (fun (u : forall (x2 : nat) (x3 : x2 ≤ q), yft0 (A0 x2 ((α ∘ !) ∘ (! ∘ x3))) x2 !)
+                      (_ : side_1 ⋅ ce_f0 (e0 q (α ∘ !)) ≡ u) =>
+                    (fun (r0 : nat) (β0 : r0 ≤ r) => ce_f0 (e0 q (α ∘ !)) r0 (side_1 ∘ (β ∘ β0))) ≡ β ⋅ u)
+                   (srefl (fun (r0 : nat) (β0 : r0 ≤ r) => ce_f0 (e0 q (α ∘ !)) r0 (side_1 ∘ (β ∘ β0))))
+                   X E))
+             (α ∘ β ⋅ x0)
+             (J_seqs _ _
+                (fun (u : forall (x2 : nat) (x3 : x2 ≤ q), yft0 (A0 x2 ((α ∘ !) ∘ (! ∘ x3))) x2 !)
+                   (_ : side_0 ⋅ ce_f0 (e0 q (α ∘ !)) ≡ u) =>
+                 (fun (r0 : nat) (β0 : r0 ≤ r) => ce_f0 (e0 q (α ∘ !)) r0 (side_0 ∘ (β ∘ β0))) ≡ β ⋅ u)
+                (srefl (fun (r0 : nat) (β0 : r0 ≤ r) => ce_f0 (e0 q (α ∘ !)) r0 (side_0 ∘ (β ∘ β0))))
+                (fun (r0 : nat) (β0 : r0 ≤ q) => x0 r0 ((α ∘ !) ∘ (! ∘ β0))) (ce_s (e0 q (α ∘ !)))))
+          (αi ∘ β)))) _ _ (ce_t (e0 q α))). simpl.
+refine (J_seqs _ _ (fun X E =>
+  yft1 (A0 q α) q !
+    (fun (r : nat) (β : r ≤ q) =>
+     cast0 A0 A1 α β
+       (itype_out
+          (J_seq (forall (x2 : nat) (x3 : x2 ≤ r), yft0 (A0 x2 ((α ∘ β) ∘ (squish ∘ (side_0 ∘ x3)))) x2 !)
+             (fun (r0 : nat) (β0 : r0 ≤ r) => ce_f0 (e0 q (α ∘ !)) r0 (promote β ∘ (side_0 ∘ β0)))
+             (fun (x : forall (x2 : nat) (x3 : x2 ≤ r), yft0 (A0 x2 ((α ∘ β) ∘ (squish ∘ (side_0 ∘ x3)))) x2 !)
+                (_ : (fun (r0 : nat) (β0 : r0 ≤ r) => ce_f0 (e0 q (α ∘ !)) r0 (promote β ∘ (side_0 ∘ β0))) ≡ x)
+              => itype r (yft0 (A0 r (α ∘ β)) r !) (x r !) (ce_f0 (e0 q (α ∘ !)) r (side_1 ∘ β)))
+             (@itype_in r (yft0 (A0 r (α ∘ β)) r !)
+                (fun αi0 : r ≤ 1 => ce_f0 (e0 q (α ∘ !)) r (promote β ∘ merge ! αi0)))
+             (β ⋅ X)
+             (J_seqs (forall (x2 : nat) (x3 : x2 ≤ q), yft0 (A0 x2 ((α ∘ !) ∘ (! ∘ x3))) x2 !)
+                (side_0 ⋅ ce_f0 (e0 q (α ∘ !)))
+                (fun (u : forall (x2 : nat) (x3 : x2 ≤ q), yft0 (A0 x2 ((α ∘ !) ∘ (! ∘ x3))) x2 !)
+                   (_ : side_0 ⋅ ce_f0 (e0 q (α ∘ !)) ≡ u) =>
+                 (fun (r0 : nat) (β0 : r0 ≤ r) => ce_f0 (e0 q (α ∘ !)) r0 (side_0 ∘ (β ∘ β0))) ≡ β ⋅ u)
+                (srefl (fun (r0 : nat) (β0 : r0 ≤ r) => ce_f0 (e0 q (α ∘ !)) r0 (side_0 ∘ (β ∘ β0))))
+                X E))
+          (αi ∘ β)))) _ _ (ce_s (e0 q α))). simpl.
+refine (J_seqs _ _
+  (fun x _ => yft1 (A0 q α) q ! (fun r β => cast0 A0 A1 α β (x r (yft0 (A0 r (α ∘ β)) r !) (fun αi0 : r ≤ 1 => ce_f0 (e0 q α) r (promote β ∘ merge ! αi0)) (αi ∘ β)))) _ _
+               (ssym itype_inout)).
+refine ((e0 q α).(ce_f1) q (merge ! αi)).
+Defined.
+
+Definition funext0 {p}
+(A0 : @El0 p Type0)
+(A1 : @El1 p Type0 Type1 A0)
+(B0 : @El0 p Type0)
+(B1 : @El1 p Type0 Type1 B0)
+(f0 : El0 (Arr0 A0 A1 B0 B1))
+(f1 : El1 _ (Arr1 A0 A1 B0 B1) f0)
+(g0 : El0 (Arr0 A0 A1 B0 B1))
+(g1 : El1 _ (Arr1 A0 A1 B0 B1) g0)
+(h0 : El0 (Prod0 A0 A1
+  (fun q α x0 x1 => eq0 (α ⋅ B0) (α ⋅ B1)
+    (app0 (α ⋅ f0) x0 x1) (app1 (α ⋅ f1) x0 x1)
+    (app0 (α ⋅ g0) x0 x1) (app1 (α ⋅ g1) x0 x1) q !)
+  (fun q α x0 x1 => eq1 (α ⋅ B0) (α ⋅ B1)
+    (app0 (α ⋅ f0) x0 x1) (app1 (α ⋅ f1) x0 x1)
+    (app0 (α ⋅ g0) x0 x1) (app1 (α ⋅ g1) x0 x1) q !)
+  ))
+(h1 : El1 _ (Prod1 A0 A1
+  (fun q α x0 x1 => eq0 (α ⋅ B0) (α ⋅ B1)
+    (app0 (α ⋅ f0) x0 x1) (app1 (α ⋅ f1) x0 x1)
+    (app0 (α ⋅ g0) x0 x1) (app1 (α ⋅ g1) x0 x1) q !)
+  (fun q α x0 x1 => eq1 (α ⋅ B0) (α ⋅ B1)
+    (app0 (α ⋅ f0) x0 x1) (app1 (α ⋅ f1) x0 x1)
+    (app0 (α ⋅ g0) x0 x1) (app1 (α ⋅ g1) x0 x1) q !)
+  ) h0)
+: El0 (eq0 (Arr0 A0 A1 B0 B1) (Arr1 A0 A1 B0 B1) f0 f1 g0 g1).
+Proof.
+unshelve refine (compare0 (Arr0 A0 A1 B0 B1) (Arr1 A0 A1 B0 B1) f0 f1 g0 g1 _ _).
+unshelve refine (path_funext0 A0 A1 B0 B1 f0 f1 g0 g1 _ _).
+refine (fun q α x0 x1 => _).
+refine (anticompare0 (α ⋅ B0) (α ⋅ B1)
+  (app0 (α ⋅ f0) x0 x1) (app1 (α ⋅ f1) x0 x1)
+  (app0 (α ⋅ g0) x0 x1) (app1 (α ⋅ g1) x0 x1)
+  (@dapp0 q (α ⋅ A0) (α ⋅ A1)
+    (fun r β y0 y1 => eq0 (α ∘ β ⋅ B0) (α ∘ β ⋅ B1)
+      (app0 (α ∘ β ⋅ f0) y0 y1) (app1 (α ∘ β ⋅ f1) y0 y1)
+      (app0 (α ∘ β ⋅ g0) y0 y1) (app1 (α ∘ β ⋅ g1) y0 y1) r !)
+    (fun r β y0 y1 => eq1 (α ∘ β ⋅ B0) (α ∘ β ⋅ B1)
+      (app0 (α ∘ β ⋅ f0) y0 y1) (app1 (α ∘ β ⋅ f1) y0 y1)
+      (app0 (α ∘ β ⋅ g0) y0 y1) (app1 (α ∘ β ⋅ g1) y0 y1) r !)
+    (α ⋅ h0) x0 x1)
+  (@dapp1 q (α ⋅ A0) (α ⋅ A1)
+    (fun r β y0 y1 => eq0 (α ∘ β ⋅ B0) (α ∘ β ⋅ B1)
+      (app0 (α ∘ β ⋅ f0) y0 y1) (app1 (α ∘ β ⋅ f1) y0 y1)
+      (app0 (α ∘ β ⋅ g0) y0 y1) (app1 (α ∘ β ⋅ g1) y0 y1) r !)
+    (fun r β y0 y1 => eq1 (α ∘ β ⋅ B0) (α ∘ β ⋅ B1)
+      (app0 (α ∘ β ⋅ f0) y0 y1) (app1 (α ∘ β ⋅ f1) y0 y1)
+      (app0 (α ∘ β ⋅ g0) y0 y1) (app1 (α ∘ β ⋅ g1) y0 y1) r !)
+    (α ⋅ h0) (α ⋅ h1) x0 x1) q !).
+refine (fun q α x0 x1 => _).
+refine (anticompare1 (α ⋅ B0) (α ⋅ B1)
+  (app0 (α ⋅ f0) x0 x1) (app1 (α ⋅ f1) x0 x1)
+  (app0 (α ⋅ g0) x0 x1) (app1 (α ⋅ g1) x0 x1)
+  (@dapp0 q (α ⋅ A0) (α ⋅ A1)
+    (fun r β y0 y1 => eq0 (α ∘ β ⋅ B0) (α ∘ β ⋅ B1)
+      (app0 (α ∘ β ⋅ f0) y0 y1) (app1 (α ∘ β ⋅ f1) y0 y1)
+      (app0 (α ∘ β ⋅ g0) y0 y1) (app1 (α ∘ β ⋅ g1) y0 y1) r !)
+    (fun r β y0 y1 => eq1 (α ∘ β ⋅ B0) (α ∘ β ⋅ B1)
+      (app0 (α ∘ β ⋅ f0) y0 y1) (app1 (α ∘ β ⋅ f1) y0 y1)
+      (app0 (α ∘ β ⋅ g0) y0 y1) (app1 (α ∘ β ⋅ g1) y0 y1) r !)
+    (α ⋅ h0) x0 x1)
+  (@dapp1 q (α ⋅ A0) (α ⋅ A1)
+  (fun r β y0 y1 => eq0 (α ∘ β ⋅ B0) (α ∘ β ⋅ B1)
+    (app0 (α ∘ β ⋅ f0) y0 y1) (app1 (α ∘ β ⋅ f1) y0 y1)
+    (app0 (α ∘ β ⋅ g0) y0 y1) (app1 (α ∘ β ⋅ g1) y0 y1) r !)
+  (fun r β y0 y1 => eq1 (α ∘ β ⋅ B0) (α ∘ β ⋅ B1)
+    (app0 (α ∘ β ⋅ f0) y0 y1) (app1 (α ∘ β ⋅ f1) y0 y1)
+    (app0 (α ∘ β ⋅ g0) y0 y1) (app1 (α ∘ β ⋅ g1) y0 y1) r !)
+  (α ⋅ h0) (α ⋅ h1) x0 x1) q !).
+unshelve refine (path_funext1 A0 A1 B0 B1 f0 f1 g0 g1
+  (fun q α x0 x1 => anticompare0 (α ⋅ B0) (α ⋅ B1)
+  (app0 (α ⋅ f0) x0 x1) (app1 (α ⋅ f1) x0 x1)
+  (app0 (α ⋅ g0) x0 x1) (app1 (α ⋅ g1) x0 x1)
+  (@dapp0 q (α ⋅ A0) (α ⋅ A1)
+    (fun r β y0 y1 => eq0 (α ∘ β ⋅ B0) (α ∘ β ⋅ B1)
+      (app0 (α ∘ β ⋅ f0) y0 y1) (app1 (α ∘ β ⋅ f1) y0 y1)
+      (app0 (α ∘ β ⋅ g0) y0 y1) (app1 (α ∘ β ⋅ g1) y0 y1) r !)
+    (fun r β y0 y1 => eq1 (α ∘ β ⋅ B0) (α ∘ β ⋅ B1)
+      (app0 (α ∘ β ⋅ f0) y0 y1) (app1 (α ∘ β ⋅ f1) y0 y1)
+      (app0 (α ∘ β ⋅ g0) y0 y1) (app1 (α ∘ β ⋅ g1) y0 y1) r !)
+    (α ⋅ h0) x0 x1)
+  (@dapp1 q (α ⋅ A0) (α ⋅ A1)
+    (fun r β y0 y1 => eq0 (α ∘ β ⋅ B0) (α ∘ β ⋅ B1)
+      (app0 (α ∘ β ⋅ f0) y0 y1) (app1 (α ∘ β ⋅ f1) y0 y1)
+      (app0 (α ∘ β ⋅ g0) y0 y1) (app1 (α ∘ β ⋅ g1) y0 y1) r !)
+    (fun r β y0 y1 => eq1 (α ∘ β ⋅ B0) (α ∘ β ⋅ B1)
+      (app0 (α ∘ β ⋅ f0) y0 y1) (app1 (α ∘ β ⋅ f1) y0 y1)
+      (app0 (α ∘ β ⋅ g0) y0 y1) (app1 (α ∘ β ⋅ g1) y0 y1) r !)
+    (α ⋅ h0) (α ⋅ h1) x0 x1) q !)
+   (fun q α x0 x1 => anticompare1 (α ⋅ B0) (α ⋅ B1)
+  (app0 (α ⋅ f0) x0 x1) (app1 (α ⋅ f1) x0 x1)
+  (app0 (α ⋅ g0) x0 x1) (app1 (α ⋅ g1) x0 x1)
+  (@dapp0 q (α ⋅ A0) (α ⋅ A1)
+    (fun r β y0 y1 => eq0 (α ∘ β ⋅ B0) (α ∘ β ⋅ B1)
+      (app0 (α ∘ β ⋅ f0) y0 y1) (app1 (α ∘ β ⋅ f1) y0 y1)
+      (app0 (α ∘ β ⋅ g0) y0 y1) (app1 (α ∘ β ⋅ g1) y0 y1) r !)
+    (fun r β y0 y1 => eq1 (α ∘ β ⋅ B0) (α ∘ β ⋅ B1)
+      (app0 (α ∘ β ⋅ f0) y0 y1) (app1 (α ∘ β ⋅ f1) y0 y1)
+      (app0 (α ∘ β ⋅ g0) y0 y1) (app1 (α ∘ β ⋅ g1) y0 y1) r !)
+    (α ⋅ h0) x0 x1)
+  (@dapp1 q (α ⋅ A0) (α ⋅ A1)
+  (fun r β y0 y1 => eq0 (α ∘ β ⋅ B0) (α ∘ β ⋅ B1)
+    (app0 (α ∘ β ⋅ f0) y0 y1) (app1 (α ∘ β ⋅ f1) y0 y1)
+    (app0 (α ∘ β ⋅ g0) y0 y1) (app1 (α ∘ β ⋅ g1) y0 y1) r !)
+  (fun r β y0 y1 => eq1 (α ∘ β ⋅ B0) (α ∘ β ⋅ B1)
+    (app0 (α ∘ β ⋅ f0) y0 y1) (app1 (α ∘ β ⋅ f1) y0 y1)
+    (app0 (α ∘ β ⋅ g0) y0 y1) (app1 (α ∘ β ⋅ g1) y0 y1) r !)
+  (α ⋅ h0) (α ⋅ h1) x0 x1) q !)).
+Defined.
+
+Definition funext1 {p}
+(A0 : @El0 p Type0)
+(A1 : @El1 p Type0 Type1 A0)
+(B0 : @El0 p Type0)
+(B1 : @El1 p Type0 Type1 B0)
+(f0 : El0 (Arr0 A0 A1 B0 B1))
+(f1 : El1 _ (Arr1 A0 A1 B0 B1) f0)
+(g0 : El0 (Arr0 A0 A1 B0 B1))
+(g1 : El1 _ (Arr1 A0 A1 B0 B1) g0)
+(h0 : El0 (Prod0 A0 A1
+  (fun q α x0 x1 => eq0 (α ⋅ B0) (α ⋅ B1)
+    (app0 (α ⋅ f0) x0 x1) (app1 (α ⋅ f1) x0 x1)
+    (app0 (α ⋅ g0) x0 x1) (app1 (α ⋅ g1) x0 x1) q !)
+  (fun q α x0 x1 => eq1 (α ⋅ B0) (α ⋅ B1)
+    (app0 (α ⋅ f0) x0 x1) (app1 (α ⋅ f1) x0 x1)
+    (app0 (α ⋅ g0) x0 x1) (app1 (α ⋅ g1) x0 x1) q !)
+  ))
+(h1 : El1 _ (Prod1 A0 A1
+  (fun q α x0 x1 => eq0 (α ⋅ B0) (α ⋅ B1)
+    (app0 (α ⋅ f0) x0 x1) (app1 (α ⋅ f1) x0 x1)
+    (app0 (α ⋅ g0) x0 x1) (app1 (α ⋅ g1) x0 x1) q !)
+  (fun q α x0 x1 => eq1 (α ⋅ B0) (α ⋅ B1)
+    (app0 (α ⋅ f0) x0 x1) (app1 (α ⋅ f1) x0 x1)
+    (app0 (α ⋅ g0) x0 x1) (app1 (α ⋅ g1) x0 x1) q !)
+  ) h0)
+: El1 _ (eq1 (Arr0 A0 A1 B0 B1) (Arr1 A0 A1 B0 B1) f0 f1 g0 g1) (funext0 A0 A1 B0 B1 f0 f1 g0 g1 h0 h1).
+Proof.
+(* TODO : just plug things together *)
+Admitted.
