theories/singletons.v
@@ -1,0 +1,225 @@
+From Theories Require Import category.
+From Theories Require Import translation_fib.
+
+Set Primitive Projections.
+Set Universe Polymorphism.
+Set Polymorphic Inductive Cumulativity.
+
+(* contractibility of singletons *)
+
+Record wedge_eq {p} 
+  (A0 : @El0 p Type0)
+  (A1 : @El1 p Type0 Type1 A0)
+  (a0 : El0 A0)
+  (a1 : El1 A0 A1 a0)
+  (b0 : El0 A0)
+  (b1 : El1 A0 A1 b0)
+  (e0 : El0 (eq0 A0 A1 a0 a1 b0 b1))
+  (e1 : El1 _ (eq1 A0 A1 a0 a1 b0 b1) e0) : Type :=
+mkWE {
+  we_f0 : @El0 (S (S p)) (squish ∘ squish ⋅ A0) ;
+  we_f1 : @El1 (S (S p)) (squish ∘ squish ⋅ A0) (squish ∘ squish ⋅ A1) we_f0 ;
+  we_0y : side_0 ⋅ we_f0 ≡ squish ⋅ a0 ;
+  we_1y : side_1 ⋅ we_f0 ≡ ce_f0 (e0 p !) ;
+  we_x0 : promote side_0 ⋅ we_f0 ≡ squish ⋅ a0 ;
+  we_x1 : promote side_1 ⋅ we_f0 ≡ ce_f0 (e0 p !) ;
+}.
+
+Arguments we_f0 {_ _ _ _ _ _ _ _ _}.
+Arguments we_f1 {_ _ _ _ _ _ _ _ _}.
+Arguments we_0y {_ _ _ _ _ _ _ _ _}.
+Arguments we_1y {_ _ _ _ _ _ _ _ _}.
+Arguments we_x0 {_ _ _ _ _ _ _ _ _}.
+Arguments we_x1 {_ _ _ _ _ _ _ _ _}.
+
+Definition we_funct {p} 
+  (A0 : @El0 p Type0)
+  (A1 : @El1 p Type0 Type1 A0)
+  (a0 : El0 A0)
+  (a1 : El1 A0 A1 a0)
+  (b0 : El0 A0)
+  (b1 : El1 A0 A1 b0)
+  (e0 : El0 (eq0 A0 A1 a0 a1 b0 b1))
+  (e1 : El1 _ (eq1 A0 A1 a0 a1 b0 b1) e0) {q} (α : q ≤ p) :
+  wedge_eq A0 A1 a0 a1 b0 b1 e0 e1 -> wedge_eq (α ⋅ A0) (α ⋅ A1) (α ⋅ a0) (α ⋅ a1) (α ⋅ b0) (α ⋅ b1) (α ⋅ e0) (α ⋅ e1).
+Proof.
+unshelve refine (fun x => _).
+unshelve econstructor.
+- exact (promote (promote α) ⋅ x.(we_f0)).
+- exact (promote (promote α) ⋅ x.(we_f1)).
+- refine (J_seqs _ _ (fun X _ => promote α ⋅ X ≡ _) (srefl _) _ (ssym (we_0y x))).
+- refine (J_seqs _ _ (fun X _ => promote α ⋅ X ≡ _) _ _ (ssym (we_1y x))).
+  refine (J_seqs _ (fun q α => ce_funct α (e0 p !)) (fun X _ => _ ≡ ce_f0 (X q α)) (srefl _) _ (ssym (e1 p !))).
+- refine (J_seqs _ _ (fun X _ => promote α ⋅ X ≡ _) (srefl _) _ (ssym (we_x0 x))).
+- refine (J_seqs _ _ (fun X _ => promote α ⋅ X ≡ _) _ _ (ssym (we_x1 x))).
+  refine (J_seqs _ (fun q α => ce_funct α (e0 p !)) (fun X _ => _ ≡ ce_f0 (X q α)) (srefl _) _ (ssym (e1 p !))).
+Defined.
+
+Definition wedge_eqR {p}
+  (A0 : @El0 p Type0)
+  (A1 : @El1 p Type0 Type1 A0)
+  (a0 : El0 A0)
+  (a1 : El1 A0 A1 a0)
+  (b0 : El0 A0)
+  (b1 : El1 A0 A1 b0)
+  (e0 : El0 (eq0 A0 A1 a0 a1 b0 b1))
+  (e1 : El1 _ (eq1 A0 A1 a0 a1 b0 b1) e0) :
+ (forall q (α : q ≤ p), wedge_eq (α ⋅ A0) (α ⋅ A1) (α ⋅ a0) (α ⋅ a1) (α ⋅ b0) (α ⋅ b1) (α ⋅ e0) (α ⋅ e1)) -> SProp :=
+fun s => s ≡ fun q α => we_funct A0 A1 a0 a1 b0 b1 e0 e1 α (s p !).
+
+Definition contractor0 {p}
+  (A0 : @El0 p Type0)
+  (A1 : @El1 p Type0 Type1 A0)
+  (a0 : El0 A0)
+  (a1 : El1 A0 A1 a0)
+  (b0 : El0 A0)
+  (b1 : El1 A0 A1 b0)
+  (e0 : El0 (eq0 A0 A1 a0 a1 b0 b1))
+  (e1 : El1 _ (eq1 A0 A1 a0 a1 b0 b1) e0)
+  : @El0 p Type0.
+Proof.
+refine (fun q α => _). unshelve econstructor.
+- unshelve refine (fun r β => _).
+  exact (wedge_eq ((α ∘ β) · A0) ((α ∘ β) · A1) ((α ∘ β) · a0) ((α ∘ β) · a1) ((α ∘ β) · b0) ((α ∘ β) · b1) ((α ∘ β) · e0) ((α ∘ β) · e1)).
+- unshelve refine (fun r β s => _). simpl in s.
+  exact (wedge_eqR ((α ∘ β) · A0) ((α ∘ β) · A1) ((α ∘ β) · a0) ((α ∘ β) · a1) ((α ∘ β) · b0) ((α ∘ β) · b1) ((α ∘ β) · e0) ((α ∘ β) · e1) s).
+- unshelve refine (fun r β b e l le l' => _).
+  apply falso.
+Defined.
+
+Definition contractor1 {p}
+  (A0 : @El0 p Type0)
+  (A1 : @El1 p Type0 Type1 A0)
+  (a0 : El0 A0)
+  (a1 : El1 A0 A1 a0)
+  (b0 : El0 A0)
+  (b1 : El1 A0 A1 b0)
+  (e0 : El0 (eq0 A0 A1 a0 a1 b0 b1))
+  (e1 : El1 _ (eq1 A0 A1 a0 a1 b0 b1) e0)
+  : @El1 p Type0 Type1 (contractor0 A0 A1 a0 a1 b0 b1 e0 e1).
+Proof.
+refine (fun q α => _).
+reflexivity.
+Defined.
+
+Definition contr_filler0 {p}
+  (A0 : @El0 p Type0)
+  (A1 : @El1 p Type0 Type1 A0)
+  (a0 : El0 A0)
+  (a1 : El1 A0 A1 a0)
+  (b0 : El0 A0)
+  (b1 : El1 A0 A1 b0)
+  (e0 : El0 (eq0 A0 A1 a0 a1 b0 b1))
+  (e1 : El1 _ (eq1 A0 A1 a0 a1 b0 b1) e0)
+  : El0 (contractor0 A0 A1 a0 a1 b0 b1 e0 e1).
+Proof.
+refine (fun q α => _). simpl. unshelve econstructor.
+- refine (wedge ⋅ ce_f0 (e0 q α)).
+- refine (wedge ⋅ ce_f1 (e0 q α)).
+- apply sfalso.
+- apply sfalso.
+- apply sfalso.
+- apply sfalso.
+(* as is, this requires some computation rules for wedge *)
+Defined.
+
+Definition contr_filler1 {p}
+  (A0 : @El0 p Type0)
+  (A1 : @El1 p Type0 Type1 A0)
+  (a0 : El0 A0)
+  (a1 : El1 A0 A1 a0)
+  (b0 : El0 A0)
+  (b1 : El1 A0 A1 b0)
+  (e0 : El0 (eq0 A0 A1 a0 a1 b0 b1))
+  (e1 : El1 _ (eq1 A0 A1 a0 a1 b0 b1) e0)
+  : El1 _ (contractor1 A0 A1 a0 a1 b0 b1 e0 e1) (contr_filler0 A0 A1 a0 a1 b0 b1 e0 e1).
+Proof.
+refine (fun q α => _).
+assert (forall (f g : forall (r : ℙ) (β : r ≤ q), wedge_eq ((α ∘ β) · A0) ((α ∘ β) · A1) ((α ∘ β) · a0) ((α ∘ β) · a1) ((α ∘ β) · b0) ((α ∘ β) · b1) ((α ∘ β) · e0) ((α ∘ β) · e1)), 
+  ((fun r β => we_f0 (f r β)) ≡ (fun r β => we_f0 (g r β))) -> f ≡ g)
+  as lemma.
+{ intros f g Hfg.
+  refine (J_seqs _ (fun r β => we_f0 (g r β)) 
+    (fun X E => (fun r β => 
+      {| we_f0 := X r β ; 
+         we_f1 := J_seqs _ _ (fun Y _ => El1 (squish ∘ squish ⋅ (α ∘ β ⋅ A0)) (squish ∘ squish ⋅ (α ∘ β ⋅ A1)) (Y r β)) (we_f1 (g r β)) _ E ;
+         we_0y := J_seqs _ (fun r β => we_f0 (g r β)) (fun Y _ => side_0 ⋅ (Y r β) ≡ squish ⋅ (α ∘ β ⋅ a0)) (we_0y (g r β)) X E ; 
+         we_1y := J_seqs _ _ (fun Y _ => side_1 ⋅ (Y r β) ≡ ce_f0 (e0 r (α ∘ β))) (we_1y (g r β)) X E ;
+         we_x0 := J_seqs _ _ (fun Y _ => (promote side_0) ⋅ (Y r β) ≡ squish ⋅ (α ∘ β ⋅ a0)) (we_x0 (g r β)) X E ;
+         we_x1 := J_seqs _ _ (fun Y _ => (promote side_1) ⋅ (Y r β) ≡ ce_f0 (e0 r (α ∘ β))) (we_x1 (g r β)) X E ; |}) 
+      ≡ g)
+    (srefl _)
+    (fun r β => we_f0 (f r β))
+    (ssym Hfg)). }
+eapply lemma. simpl.
+refine (J_seqs _ _ (fun X _ => (fun r β => wedge ⋅ ce_f0 (X r β)) ≡ _) (srefl _) (α ⋅ e0) (ssym (e1 q α))).
+Defined.
+
+
+(* that one is more or less contr_filler0 with some packaging *)
+(* todo : prove it from contr_filler0 *)
+Definition singl_contr0 {p}
+  (A0 : @El0 p Type0)
+  (A1 : @El1 p Type0 Type1 A0)
+  (a0 : El0 A0)
+  (a1 : El1 A0 A1 a0)
+  (b0 : El0 A0)
+  (b1 : El1 A0 A1 b0)
+  (e0 : El0 (eq0 A0 A1 a0 a1 b0 b1))
+  (e1 : El1 _ (eq1 A0 A1 a0 a1 b0 b1) e0)
+  : El0 (eq0
+    (Sigma0 A0 A1 (fun q α x0 x1 => eq0 (α ⋅ A0) (α ⋅ A1) (α ⋅ a0) (α ⋅ a1) x0 x1 q !) (fun q α x0 x1 => eq1 (α ⋅ A0) (α ⋅ A1) (α ⋅ a0) (α ⋅ a1) x0 x1 q !))
+    (Sigma1 A0 A1 (fun q α x0 x1 => eq0 (α ⋅ A0) (α ⋅ A1) (α ⋅ a0) (α ⋅ a1) x0 x1 q !) (fun q α x0 x1 => eq1 (α ⋅ A0) (α ⋅ A1) (α ⋅ a0) (α ⋅ a1) x0 x1 q !))
+    (dpair0 a0 a1 (eq_refl0 A0 A1 a0 a1) (eq_refl1 A0 A1 a0 a1))
+    (dpair1 a0 a1 (eq_refl0 A0 A1 a0 a1) (eq_refl1 A0 A1 a0 a1))
+    (dpair0 b0 b1 e0 e1)
+    (dpair1 b0 b1 e0 e1)).
+Proof.
+refine (fun q α => _) ; simpl.
+unshelve econstructor.
+- refine (fun r β => _) ; simpl.
+  unshelve econstructor.
+  + exact (β ⋅ ce_f0 (e0 q α)).
+  + exact (β ⋅ ce_f1 (e0 q α)).
+  + refine (fun r0 β0 => _) ; simpl.
+    unshelve econstructor.
+    * change (El0 (α ∘ squish ∘ wedge ∘ promote β ∘ promote β0 ⋅ A0)).
+      exact (wedge ∘ promote β ∘ promote β0 ⋅ (ce_f0 (e0 q α))).
+    * exact (wedge ∘ promote β ∘ promote β0 ⋅ (ce_f1 (e0 q α))).
+    * refine (J_seqs _ _ (fun X _ => _ ≡ β ∘ β0 ⋅ (squish ⋅ X)) _ _ (ce_s (e0 q α))).
+      change (β ∘ β0 ⋅ (wedge ∘ side_0 ⋅ ce_f0 (e0 q α)) ≡ β ∘ β0 ⋅ (side_0 ∘ squish ⋅ (ce_f0 (e0 q α)))).
+      (* here we would need some more computation *)
+      apply sfalso.
+    * change (β ∘ β0 ⋅ (wedge ∘ side_1 ⋅ ce_f0 (e0 q α)) ≡ β ∘ β0 ⋅ (ce_f0 (e0 q α))).
+      (* here too *)
+      apply sfalso.
+  + refine (fun r0 β0 => _) ; simpl.
+    reflexivity.
+- refine (fun r β => _) ; simpl.
+  reflexivity.
+- admit.
+- admit.
+Admitted.
+
+
+Definition singl_contr1 {p}
+  (A0 : @El0 p Type0)
+  (A1 : @El1 p Type0 Type1 A0)
+  (a0 : El0 A0)
+  (a1 : El1 A0 A1 a0)
+  (b0 : El0 A0)
+  (b1 : El1 A0 A1 b0)
+  (e0 : El0 (eq0 A0 A1 a0 a1 b0 b1))
+  (e1 : El1 _ (eq1 A0 A1 a0 a1 b0 b1) e0)
+  : El1 _ (eq1
+    (Sigma0 A0 A1 (fun q α x0 x1 => eq0 (α ⋅ A0) (α ⋅ A1) (α ⋅ a0) (α ⋅ a1) x0 x1 q !) (fun q α x0 x1 => eq1 (α ⋅ A0) (α ⋅ A1) (α ⋅ a0) (α ⋅ a1) x0 x1 q !))
+    (Sigma1 A0 A1 (fun q α x0 x1 => eq0 (α ⋅ A0) (α ⋅ A1) (α ⋅ a0) (α ⋅ a1) x0 x1 q !) (fun q α x0 x1 => eq1 (α ⋅ A0) (α ⋅ A1) (α ⋅ a0) (α ⋅ a1) x0 x1 q !))
+    (dpair0 a0 a1 (eq_refl0 A0 A1 a0 a1) (eq_refl1 A0 A1 a0 a1))
+    (dpair1 a0 a1 (eq_refl0 A0 A1 a0 a1) (eq_refl1 A0 A1 a0 a1))
+    (dpair0 b0 b1 e0 e1)
+    (dpair1 b0 b1 e0 e1))
+    (singl_contr0 A0 A1 a0 a1 b0 b1 e0 e1).
+Proof.
+refine (fun q α => _). simpl.
+(* komarimasu… *)
+Admitted.
