theories/transport.v
@@ -1,0 +1,304 @@
+From Theories Require Import category.
+From Theories Require Import translation_fib.
+
+Set Primitive Projections.
+Set Universe Polymorphism.
+Set Polymorphic Inductive Cumulativity.
+
+(* shifted types *)
+
+Record shifted_ty {p} : Type :=
+mkST {
+  st_t0 : @El0 (S p) (squish ⋅ Type0) ;
+  st_t1 : @El1 (S p) (squish ⋅ Type0) (squish ⋅ Type1) st_t0 ;
+}.
+
+Definition st_funct {p} {q} (α : q ≤ p) :
+  @shifted_ty p -> @shifted_ty q.
+Proof.
+unshelve refine (fun x => _).
+unshelve econstructor.
+- exact (promote α ⋅ x.(st_t0)).
+- exact (promote α ⋅ x.(st_t1)).
+Defined.
+
+Definition shifted_tyR {p} :
+ (forall q (α : q ≤ p), @shifted_ty q) -> SProp :=
+fun s => s ≡ fun q α => st_funct α (s p !).
+
+Definition shiftedType0 {p}
+  : @El0 p Type0.
+Proof.
+unshelve refine (fun q α => mkYFT _ _ _ _).
+- unshelve refine (fun r β => _).
+  exact (@shifted_ty r).
+- unshelve refine (fun r β s => _). simpl in s.
+  exact (shifted_tyR s).
+- unshelve refine (fun r β b e l le l' => _).
+  apply falso. (** TODO **)
+Defined.
+
+Definition shiftedType1 {p}
+  : @El1 p Type0 Type1 shiftedType0.
+Proof.
+refine (fun q α => _). reflexivity.
+Defined.
+
+Definition shiftedTypeStart0 {p}
+  (A0 : @El0 p shiftedType0)
+  (A1 : @El1 p shiftedType0 shiftedType1 A0) :
+  @El0 p Type0.
+Proof.
+refine (fun q α => _).
+refine ((side_0 ⋅ st_t0 (A0 q α)) q !). 
+Defined.
+
+Definition shiftedTypeStart1 {p}
+  (A0 : @El0 p shiftedType0)
+  (A1 : @El1 p shiftedType0 shiftedType1 A0) :
+  @El1 p Type0 Type1 (shiftedTypeStart0 A0 A1).
+Proof.
+refine (fun q α => _). 
+refine (J_seqs _ _ (fun X _ => yftR (fun r β => st_t0 (X r β) r side_0 )) _ (α ⋅ A0) (ssym (A1 q α))).
+refine ((side_0 ⋅ st_t1 (A0 q α)) q !).
+Defined.
+
+Definition shiftedTypeEnd0 {p}
+  (A0 : @El0 p shiftedType0)
+  (A1 : @El1 p shiftedType0 shiftedType1 A0) :
+  @El0 p Type0.
+Proof.
+refine (fun q α => _).
+refine ((side_1 ⋅ st_t0 (A0 q α)) q !). 
+Defined.
+
+Definition shiftedTypeEnd1 {p}
+  (A0 : @El0 p shiftedType0)
+  (A1 : @El1 p shiftedType0 shiftedType1 A0) :
+  @El1 p Type0 Type1 (shiftedTypeEnd0 A0 A1).
+Proof.
+refine (fun q α => _). 
+refine (J_seqs _ _ (fun X _ => yftR (fun r β => st_t0 (X r β) r side_1)) _ (α ⋅ A0) (ssym (A1 q α))).
+refine ((side_1 ⋅ st_t1 (A0 q α)) q !).
+Defined.
+
+(* a predicate over an equality is a shifted type *)
+
+Definition eqToShiftedType0 {p}
+  (A0 : @El0 p Type0)
+  (A1 : @El1 p Type0 Type1 A0)
+  (P0 : El0 (Arr0 A0 A1 Type0 Type1))
+  (P1 : El1 _ (Arr1 A0 A1 Type0 Type1) P0)
+  (a0 : El0 A0)
+  (a1 : El1 A0 A1 a0)
+  (b0 : El0 A0)
+  (b1 : El1 A0 A1 b0)
+  (e0 : El0 (eq0 A0 A1 a0 a1 b0 b1))
+  (e1 : El1 _ (eq1 A0 A1 a0 a1 b0 b1) e0) :
+  @El0 p shiftedType0.
+Proof.
+refine (fun q α => _).
+unshelve econstructor.
+- refine (fun r β => P0 r (α ∘ squish ∘ β) (β ⋅ (ce_f0 (e0 q α))) (β ⋅ ce_f1 (e0 q α))).
+- refine (@app1 (S q) _ _ Type0 Type1 (α ∘ squish ⋅ P0) (α ∘ squish ⋅ P1) (ce_f0 (e0 q α)) (ce_f1 (e0 q α))).
+Defined.
+
+Definition eqToShiftedType1 {p}
+  (A0 : @El0 p Type0)
+  (A1 : @El1 p Type0 Type1 A0)
+  (P0 : El0 (Arr0 A0 A1 Type0 Type1))
+  (P1 : El1 _ (Arr1 A0 A1 Type0 Type1) P0)
+  (a0 : El0 A0)
+  (a1 : El1 A0 A1 a0)
+  (b0 : El0 A0)
+  (b1 : El1 A0 A1 b0)
+  (e0 : El0 (eq0 A0 A1 a0 a1 b0 b1))
+  (e1 : El1 _ (eq1 A0 A1 a0 a1 b0 b1) e0) :
+  @El1 p shiftedType0 shiftedType1 (eqToShiftedType0 A0 A1 P0 P1 a0 a1 b0 b1 e0 e1).
+Proof.
+refine (fun q α => _).
+unfold cast0 ; simpl. unfold shifted_tyR ; simpl.
+change (eqToShiftedType0 (α ⋅ A0) (α ⋅ A1) (α ⋅ P0) (α ⋅ P1) (α ⋅ a0) (α ⋅ a1) (α ⋅ b0) (α ⋅ b1) (α ⋅ e0) (α ⋅ e1) ≡ (fun r β => st_funct β (eqToShiftedType0 A0 A1 P0 P1 a0 a1 b0 b1 e0 e1 q α))).
+pose proof (e1 q α) as He. unfold cast0 in He ; simpl in He.
+unfold cube_eqR in He.
+refine (J_seqs _ _ 
+  (fun X e => eqToShiftedType0 _ _ _ _ _ _ _ _ X 
+    (J_seqs _ _ (fun Y _ => El1 _ (eq1 (α ⋅ A0) (α ⋅ A1) (α ⋅ a0) (α ⋅ a1) (α ⋅ b0) (α ⋅ b1)) Y) 
+      (J_seqs _ (α ⋅ e0) (fun Z _ => El1 _ (eq1 (α ⋅ A0) (α ⋅ A1) (α ⋅ a0) (α ⋅ a1) (α ⋅ b0) (α ⋅ b1)) Z) (α ⋅ e1) _ He) 
+      X e) 
+    ≡ _) 
+  _ (α ⋅ e0) (ssym He)).
+reflexivity.
+Defined.
+
+(* transport boils down to a statement about shifted types *)
+
+Definition transp0 {p}
+  (A0 : @El0 p shiftedType0)
+  (A1 : @El1 p shiftedType0 shiftedType1 A0)
+  (s0 : El0 (shiftedTypeStart0 A0 A1))
+  (s1 : El1 _ (shiftedTypeStart1 A0 A1) s0)
+  : El0 (shiftedTypeEnd0 A0 A1).
+Proof.
+refine (fun q α => _).
+unfold shiftedTypeEnd0 ; simpl.
+unfold El0 in s0 ; unfold shiftedTypeStart0 in s0 ; simpl in s0. 
+change (forall q α, yft0 (st_t0 (A0 q α) q side_0) q !) in s0.
+unfold El0 in A0 ; simpl in A0.
+
+refine (J_seq _ _ (fun X _ => yft0 (X q side_1) q !) _ _ (ssym (st_t1 (A0 q α) (S q) !))).
+change (yft0 (st_t0 (A0 q α) (S q) !) q side_1).
+
+unshelve refine (let s'0 : yft0 (st_t0 (A0 q α) (S q) !) q side_0 := _ in _).
+{ pose proof (st_t1 (A0 q α) (S q) !) as H. change (yftR (st_t0 (A0 q α))) in H. unfold yftR in H.
+  refine (J_seq _ _ (fun X _ => yft0 (X q side_0) q !) _ _ H).
+  refine (s0 q α). }
+
+Admitted.
+
+Definition transp1 {p}
+  (A0 : @El0 p shiftedType0)
+  (A1 : @El1 p shiftedType0 shiftedType1 A0)
+  (s0 : El0 (shiftedTypeStart0 A0 A1))
+  (s1 : El1 _ (shiftedTypeStart1 A0 A1) s0)
+  : El1 _ (shiftedTypeEnd1 A0 A1) (transp0 A0 A1 s0 s1).
+Proof.
+Admitted.
+
+Definition transport_aux1_0 {p}
+  (A0 : @El0 p Type0)
+  (A1 : @El1 p Type0 Type1 A0)
+  (P0 : El0 (Arr0 A0 A1 Type0 Type1))
+  (P1 : El1 _ (Arr1 A0 A1 Type0 Type1) P0)
+  (a0 : El0 A0)
+  (a1 : El1 A0 A1 a0)
+  (x0 : El0 (app0 P0 a0 a1))
+  (x1 : El1 _ (app1 P1 a0 a1) x0)
+  (b0 : El0 A0)
+  (b1 : El1 A0 A1 b0)
+  (e0 : El0 (eq0 A0 A1 a0 a1 b0 b1))
+  (e1 : El1 _ (eq1 A0 A1 a0 a1 b0 b1) e0) :
+  El0 (shiftedTypeStart0 (eqToShiftedType0 A0 A1 P0 P1 a0 a1 b0 b1 e0 e1) (eqToShiftedType1 A0 A1 P0 P1 a0 a1 b0 b1 e0 e1)).
+Proof.
+refine (fun q α => _).
+change (yft0 (P0 q α (side_0 ⋅ ce_f0 (e0 q α)) (side_0 ⋅ ce_f1 (e0 q α))) q !).
+refine (J_seq _ (α ⋅ a0) 
+  (fun X E => yft0 (P0 q α X 
+    (J_seqs _ _ (fun Y _ => El1 (α ⋅ A0) (α ⋅ A1) Y) (α ⋅ a1) X E)) 
+    q !)
+  _ _ (ssym (ce_s (e0 q α)))).
+refine (x0 q α).
+Defined.
+
+Definition transport_aux1_1 {p}
+  (A0 : @El0 p Type0)
+  (A1 : @El1 p Type0 Type1 A0)
+  (P0 : El0 (Arr0 A0 A1 Type0 Type1))
+  (P1 : El1 _ (Arr1 A0 A1 Type0 Type1) P0)
+  (a0 : El0 A0)
+  (a1 : El1 A0 A1 a0)
+  (x0 : El0 (app0 P0 a0 a1))
+  (x1 : El1 _ (app1 P1 a0 a1) x0)
+  (b0 : El0 A0)
+  (b1 : El1 A0 A1 b0)
+  (e0 : El0 (eq0 A0 A1 a0 a1 b0 b1))
+  (e1 : El1 _ (eq1 A0 A1 a0 a1 b0 b1) e0) :
+  El1 _ (shiftedTypeStart1 (eqToShiftedType0 A0 A1 P0 P1 a0 a1 b0 b1 e0 e1) (eqToShiftedType1 A0 A1 P0 P1 a0 a1 b0 b1 e0 e1)) (transport_aux1_0 A0 A1 P0 P1 a0 a1 x0 x1 b0 b1 e0 e1).
+Proof.
+refine (fun q α => _). 
+unfold transport_aux1_0 ; simpl.
+unfold shiftedTypeStart0 ; unfold eqToShiftedType0 at 1 2 ; simpl.
+(* unfolding shiftedTypeStart1 unleashes hell *)
+Admitted.
+
+Definition transport_aux2_0 {p}
+  (A0 : @El0 p Type0)
+  (A1 : @El1 p Type0 Type1 A0)
+  (P0 : El0 (Arr0 A0 A1 Type0 Type1))
+  (P1 : El1 _ (Arr1 A0 A1 Type0 Type1) P0)
+  (a0 : El0 A0)
+  (a1 : El1 A0 A1 a0)
+  (b0 : El0 A0)
+  (b1 : El1 A0 A1 b0)
+  (e0 : El0 (eq0 A0 A1 a0 a1 b0 b1))
+  (e1 : El1 _ (eq1 A0 A1 a0 a1 b0 b1) e0)
+  (x0 : El0 (shiftedTypeEnd0 (eqToShiftedType0 A0 A1 P0 P1 a0 a1 b0 b1 e0 e1) (eqToShiftedType1 A0 A1 P0 P1 a0 a1 b0 b1 e0 e1)))
+  (x1 : El1 _ (shiftedTypeEnd1 (eqToShiftedType0 A0 A1 P0 P1 a0 a1 b0 b1 e0 e1) (eqToShiftedType1 A0 A1 P0 P1 a0 a1 b0 b1 e0 e1)) x0) :
+  El0 (app0 P0 b0 b1).
+Proof.
+refine (fun q α => _).
+change (yft0 (P0 q α (α ⋅ b0) (α ⋅ b1)) q !).
+refine (J_seq _ _ 
+  (fun X E => yft0 (P0 q α X 
+    (J_seqs _ _ (fun Y _ => El1 (α ⋅ A0) (α ⋅ A1) Y) 
+      (J_seqs _ (α ⋅ b0) (fun Z _ => El1 (α ⋅ A0) (α ⋅ A1) Z) (α ⋅ b1) _ (ssym (ce_t (e0 q α)))) X E)) 
+    q !)
+  _ (α ⋅ b0) (ce_t (e0 q α))).
+change (yft0 (P0 q α (side_1 ⋅ ce_f0 (e0 q α)) (side_1 ⋅ ce_f1 (e0 q α))) q !).
+refine (x0 q α).
+Defined.
+
+Definition transport_aux2_1 {p}
+  (A0 : @El0 p Type0)
+  (A1 : @El1 p Type0 Type1 A0)
+  (P0 : El0 (Arr0 A0 A1 Type0 Type1))
+  (P1 : El1 _ (Arr1 A0 A1 Type0 Type1) P0)
+  (a0 : El0 A0)
+  (a1 : El1 A0 A1 a0)
+  (b0 : El0 A0)
+  (b1 : El1 A0 A1 b0)
+  (e0 : El0 (eq0 A0 A1 a0 a1 b0 b1))
+  (e1 : El1 _ (eq1 A0 A1 a0 a1 b0 b1) e0)
+  (x0 : El0 (shiftedTypeEnd0 (eqToShiftedType0 A0 A1 P0 P1 a0 a1 b0 b1 e0 e1) (eqToShiftedType1 A0 A1 P0 P1 a0 a1 b0 b1 e0 e1)))
+  (x1 : El1 _ (shiftedTypeEnd1 (eqToShiftedType0 A0 A1 P0 P1 a0 a1 b0 b1 e0 e1) (eqToShiftedType1 A0 A1 P0 P1 a0 a1 b0 b1 e0 e1)) x0) :
+  El1 (app0 P0 b0 b1) (app1 P1 b0 b1) (transport_aux2_0 A0 A1 P0 P1 a0 a1 b0 b1 e0 e1 x0 x1).
+Proof.
+Admitted.
+
+Definition transport0 {p}
+  (A0 : @El0 p Type0)
+  (A1 : @El1 p Type0 Type1 A0)
+  (P0 : El0 (Arr0 A0 A1 Type0 Type1))
+  (P1 : El1 _ (Arr1 A0 A1 Type0 Type1) P0)
+  (a0 : El0 A0)
+  (a1 : El1 A0 A1 a0)
+  (x0 : El0 (app0 P0 a0 a1))
+  (x1 : El1 _ (app1 P1 a0 a1) x0)
+  (b0 : El0 A0)
+  (b1 : El1 A0 A1 b0)
+  (e0 : El0 (eq0 A0 A1 a0 a1 b0 b1))
+  (e1 : El1 _ (eq1 A0 A1 a0 a1 b0 b1) e0) :
+  El0 (app0 P0 b0 b1).
+Proof.
+refine (transport_aux2_0 A0 A1 P0 P1 a0 a1 b0 b1 e0 e1 
+  (transp0 (eqToShiftedType0 A0 A1 P0 P1 a0 a1 b0 b1 e0 e1) (eqToShiftedType1 A0 A1 P0 P1 a0 a1 b0 b1 e0 e1)
+    (transport_aux1_0 A0 A1 P0 P1 a0 a1 x0 x1 b0 b1 e0 e1)
+    (transport_aux1_1 A0 A1 P0 P1 a0 a1 x0 x1 b0 b1 e0 e1))
+  (transp1 (eqToShiftedType0 A0 A1 P0 P1 a0 a1 b0 b1 e0 e1) (eqToShiftedType1 A0 A1 P0 P1 a0 a1 b0 b1 e0 e1)
+    (transport_aux1_0 A0 A1 P0 P1 a0 a1 x0 x1 b0 b1 e0 e1)
+    (transport_aux1_1 A0 A1 P0 P1 a0 a1 x0 x1 b0 b1 e0 e1))).
+Defined.
+
+Definition transport1 {p}
+  (A0 : @El0 p Type0)
+  (A1 : @El1 p Type0 Type1 A0)
+  (P0 : El0 (Arr0 A0 A1 Type0 Type1))
+  (P1 : El1 _ (Arr1 A0 A1 Type0 Type1) P0)
+  (a0 : El0 A0)
+  (a1 : El1 A0 A1 a0)
+  (x0 : El0 (app0 P0 a0 a1))
+  (x1 : El1 _ (app1 P1 a0 a1) x0)
+  (b0 : El0 A0)
+  (b1 : El1 A0 A1 b0)
+  (e0 : El0 (eq0 A0 A1 a0 a1 b0 b1))
+  (e1 : El1 _ (eq1 A0 A1 a0 a1 b0 b1) e0) :
+  El1 (app0 P0 b0 b1) (app1 P1 b0 b1) (transport0 A0 A1 P0 P1 a0 a1 x0 x1 b0 b1 e0 e1).
+Proof.
+refine (transport_aux2_1 A0 A1 P0 P1 a0 a1 b0 b1 e0 e1 
+  (transp0 (eqToShiftedType0 A0 A1 P0 P1 a0 a1 b0 b1 e0 e1) (eqToShiftedType1 A0 A1 P0 P1 a0 a1 b0 b1 e0 e1)
+    (transport_aux1_0 A0 A1 P0 P1 a0 a1 x0 x1 b0 b1 e0 e1)
+    (transport_aux1_1 A0 A1 P0 P1 a0 a1 x0 x1 b0 b1 e0 e1))
+  (transp1 (eqToShiftedType0 A0 A1 P0 P1 a0 a1 b0 b1 e0 e1) (eqToShiftedType1 A0 A1 P0 P1 a0 a1 b0 b1 e0 e1)
+    (transport_aux1_0 A0 A1 P0 P1 a0 a1 x0 x1 b0 b1 e0 e1)
+    (transport_aux1_1 A0 A1 P0 P1 a0 a1 x0 x1 b0 b1 e0 e1))).
+Defined.
