theories/univalence.v
@@ -1,0 +1,38 @@
+From Theories Require Import category.
+From Theories Require Import translation_fib.
+
+Set Primitive Projections.
+Set Universe Polymorphism.
+Set Polymorphic Inductive Cumulativity.
+
+(* weak univalence *)
+(* for now lets just try to glue bool along bool... *)
+
+(* Definition glueType (p : ℙ) (A B : Type) : itype p Type A B.
+Proof.
+refine (J_seq _ (glueTypeAux p A B i0) (fun X _ => itype p Type X B) _ _ (glueTypeAux_i0)).
+refine (J_seq _ (glueTypeAux p A B i1) (fun X _ => itype p Type (glueTypeAux p A B i0) X) _ _ (glueTypeAux_i1)).
+refine (itype_in (glueTypeAux p A B)).
+Defined.
+
+Definition weakunivalence0 {p}
+  (A0 : @El0 p Type0)
+  (A1 : @El1 p Type0 Type1 A0)
+  (B0 : @El0 p Type0)
+  (B1 : @El1 p Type0 Type1 B0)
+  : El0 (eq0 Type0 Type1 A0 A1 B0 B1).
+Proof.
+refine (fun q α => _).
+unshelve econstructor.
+- refine (fun r β => _).
+  unshelve econstructor.
+  + refine (fun r0 β0 => _).
+    refine (itype_out (glueType r0 (yft0 (A0 r0 (α ∘ squish ∘ β ∘ β0)) r0 !) (yft0 (B0 r0 (α ∘ squish ∘ β ∘ β0)) r0 !)) (antisquish ∘ β ∘ β0)).
+  + refine (fun r0 β0 s => _) ; simpl in s.
+    admit.
+  + refine (fun r0 β0 a b c d e => _).
+    admit.
+- refine (fun r β r0 β0 => _). unfold cast0 ; simpl. reflexivity.
+- simpl.
+Admitted. *)
+
